examples/crypto/OPLSS.AE.fst
@@ -1,0 +1,286 @@
+(*
+   Copyright 2008-2018 Microsoft Research
+
+   Licensed under the Apache License, Version 2.0 (the "License");
+   you may not use this file except in compliance with the License.
+   You may obtain a copy of the License at
+
+       http://www.apache.org/licenses/LICENSE-2.0
+
+   Unless required by applicable law or agreed to in writing, software
+   distributed under the License is distributed on an "AS IS" BASIS,
+   WITHOUT WARRANTIES OR CONDITIONS OF ANY KIND, either express or implied.
+   See the License for the specific language governing permissions and
+   limitations under the License.
+*)
+module OPLSS.AE
+open FStar.Seq
+open FStar.HyperStack
+open FStar.HyperStack.ST
+
+module MAC = OPLSS.MAC
+module CPA = OPLSS.CPA
+module Ideal = OPLSS.Ideal
+module Plain = OPLSS.Plain
+module B = LowStar.Monotonic.Buffer
+
+(*** Basic types ***)
+
+
+/// An AE key pairs an encryption key, ke, with a MAC'ing key, km,
+/// with an invariant ensuring that their memory footprints of their
+/// ideal state are disjoint.
+/// 
+/// Aside from this, we have an AE log, which is a view of the two
+/// other logs.
+noeq type key =
+  | Key: mac:MAC.key
+       -> enc:CPA.key { 
+           B.loc_disjoint (B.loc_mreference mac.MAC.log)
+                          (B.loc_mreference enc.CPA.log)
+           }
+       -> key
+
+/// mac log
+let mac_log (h:mem) (k:key) =
+  sel h k.mac.MAC.log
+
+/// cpa log
+let cpa_log (h:mem) (k:key) =
+  sel h k.enc.CPA.log
+
+(*** Main invariant on the ideal state ***)
+(** There are two main components to this invariant
+
+     1. mac_only_cpa_ciphers: 
+       
+        The MAC log and CPA logs are related, in that the MAC log only
+        contains entries for valid ciphers recorded the CPA log
+
+     2. The CPA invariant (pairwise distinctness of IVs, notably)
+**)
+
+let mac_cpa_related (mac:MAC.log_entry) (enc:CPA.log_entry) =
+  mac.MAC.msg == enc.CPA.c
+
+/// See the comment above, for part 2 of the invariant
+///   -- As in EtM.CPA, we state the invariant recursively
+///      matching entries up pointwise
+let rec mac_only_cpa_ciphers (macs:Seq.seq MAC.log_entry) 
+                             (cpas:Seq.seq CPA.log_entry)
+      : Tot Type0 (decreases (Seq.length macs)) =
+   Seq.length macs == Seq.length cpas /\
+   (if Seq.length macs > 0 then
+     let macs, mac = Seq.un_snoc macs in
+     let cpas, cpa = Seq.un_snoc cpas in
+     mac_cpa_related mac cpa /\
+     mac_only_cpa_ciphers macs cpas
+    else True)
+
+/// A lemma to intro/elim the recursive predicate above
+let mac_only_cpa_ciphers_snoc (macs:Seq.seq MAC.log_entry) (mac:MAC.log_entry)
+                              (cpas:Seq.seq CPA.log_entry) (cpa:CPA.log_entry)
+  : Lemma (mac_only_cpa_ciphers (snoc macs mac) (snoc cpas cpa) <==>
+          (mac_only_cpa_ciphers macs cpas /\ mac_cpa_related mac cpa))
+  = un_snoc_snoc macs mac;
+    un_snoc_snoc cpas cpa
+
+let ae_cipher = AES.iv_cipher * MAC.tag
+let ae_as_mac (c:ae_cipher) = MAC.Entry (fst c) (snd c)
+
+/// A lemma that shows that if a cipher is MAC'd
+/// then a corresponding entry must exists in the CPA log
+let rec mac_only_cpa_ciphers_mem (macs:Seq.seq MAC.log_entry) 
+                                 (cpas:Seq.seq CPA.log_entry)
+                                 (c:ae_cipher)
+    : Lemma (requires (mac_only_cpa_ciphers macs cpas /\
+                       Seq.mem (ae_as_mac c) macs))
+            (ensures (exists p. Seq.mem (CPA.Entry p (fst c)) cpas))
+            (decreases (Seq.length macs))
+    = if Seq.length macs = 0 then
+         ()
+      else let macs, mac = un_snoc macs in
+           let cpas, cpa = un_snoc cpas in
+           Seq.lemma_mem_snoc macs mac;
+           Seq.lemma_mem_snoc cpas cpa;
+           if mac = ae_as_mac c then ()
+           else mac_only_cpa_ciphers_mem macs cpas c
+
+let ae = Ideal.uf_cma
+
+/// The main invariant:
+///     -- A conjunction of the 3 components already mentioned
+///      + some technical invariants about logs being allocated
+let invariant k h =
+  CPA.invariant k.enc h /\
+  MAC.invariant k.mac h /\
+  (ae ==> mac_only_cpa_ciphers (mac_log h k) (cpa_log h k))
+
+let log_entry = Plain.plain & ae_cipher
+
+let composite_log_entry (mac:MAC.log_entry) (cpa:CPA.log_entry) : log_entry =
+  (cpa.CPA.plain, (cpa.CPA.c, mac.MAC.tag))  
+  
+let rec composite_log (macs:Seq.seq MAC.log_entry) 
+                      (cpas:Seq.seq CPA.log_entry{mac_only_cpa_ciphers macs cpas})
+  : Tot (aes:Seq.seq log_entry{Seq.length aes = Seq.length macs}) (decreases (Seq.length macs))
+  = if Seq.length macs = 0 then Seq.empty
+    else let macs, mac = un_snoc macs in
+         let cpas, cpa = un_snoc cpas in
+         Seq.snoc (composite_log macs cpas) (composite_log_entry mac cpa)
+
+let composite_log_snoc
+       (macs:Seq.seq MAC.log_entry) 
+       (mac:MAC.log_entry)
+       (cpas:Seq.seq CPA.log_entry)
+       (cpa:CPA.log_entry{
+         mac_only_cpa_ciphers macs cpas /\
+         mac_only_cpa_ciphers (snoc macs mac) (snoc cpas cpa)})
+  : Lemma (composite_log (snoc macs mac) (snoc cpas cpa) ==
+           snoc (composite_log macs cpas) (composite_log_entry mac cpa))
+  = un_snoc_snoc macs mac;
+    un_snoc_snoc cpas cpa
+
+let ae_log (k:key) (h:mem{invariant k h /\ ae}) =
+  composite_log (MAC.log k.mac h) (CPA.log k.enc h)
+
+(*** The main AE lemma relying on the invariant  ***)
+
+(** For logs that respect the main invariant:
+//        if  (c, t) is a valid MAC
+//        and (p, c) is a valid CPA
+//        then (p, (c, t)) must be a in the AE log
+
+//     The pairwise distinctness of ciphers in the CPA log
+//     plays a crucial role.
+
+//     For instance, using it, and knowing that (c, t) is a valid MAC, 
+//     we can conclude that their must be exactly one entry 
+//     in the CPA table containing c. **)
+let rec invert_invariant_aux (macs:Seq.seq MAC.log_entry)
+                             (cpas:Seq.seq CPA.log_entry)
+                             (c:ae_cipher) (p:Plain.plain)
+   : Lemma 
+     (requires 
+       mac_only_cpa_ciphers macs cpas /\
+       CPA.pairwise_distinct_ivs cpas /\
+       Seq.mem (ae_as_mac c) macs /\
+       Seq.mem (CPA.Entry p (fst c)) cpas)
+     (ensures
+       Seq.mem (p, c) (composite_log macs cpas))
+     (decreases (Seq.length macs))
+   = let aes = composite_log macs cpas in
+     assert (Seq.length macs == Seq.length aes);
+     if Seq.length macs = 0 then ()
+     else let macs, mac = un_snoc macs in
+          let cpas, cpa = un_snoc cpas in
+          assert (CPA.pairwise_distinct_ivs (snoc cpas cpa));          
+          let aes,   ae = un_snoc aes  in
+          Seq.lemma_mem_snoc aes ae;
+          Seq.lemma_mem_snoc macs mac;
+          Seq.lemma_mem_snoc cpas cpa;
+           if mac = ae_as_mac c then begin
+             assert (cpa.CPA.c == fst c);
+             CPA.invert_pairwise cpas cpa (fst c);
+             assert (not (Seq.mem (CPA.Entry p (fst c)) cpas));
+             assert (CPA.Entry?.plain cpa == p);
+             assert (ae = (p, c))
+           end
+           else if mac.MAC.msg = fst c then begin
+             assert (CPA.Entry?.c cpa == fst c);
+             mac_only_cpa_ciphers_mem macs cpas c;
+             assert (exists q1. Seq.mem (CPA.Entry q1 (fst c)) cpas);
+             CPA.invert_pairwise cpas cpa (fst c)
+           end
+           else begin
+             mac_only_cpa_ciphers_snoc macs mac cpas cpa;
+             CPA.pairwise_snoc cpas cpa;
+             invert_invariant_aux macs cpas c p;
+             assert (Seq.mem (p, c) (composite_log macs cpas));
+             composite_log_snoc macs mac cpas cpa;
+             Seq.lemma_mem_snoc (composite_log macs cpas) (composite_log_entry mac cpa)
+           end
+
+/// Lifting the lemma above to work on the current state, h
+let invert_invariant (h:mem) (k:key) (c:ae_cipher) (p:Plain.plain)
+  : Lemma 
+    (requires 
+      ae /\
+      invariant k h /\
+      Seq.mem (ae_as_mac c) (mac_log h k) /\
+      Seq.mem (CPA.Entry p (fst c)) (cpa_log h k))
+    (ensures 
+      Seq.mem (p, c) (ae_log k h))
+    = let macs = mac_log h k in
+      let cpas = cpa_log h k in
+      let aes  = ae_log k h in
+      invert_invariant_aux macs cpas c p
+
+(*** Main interface of AE
+     keygen, encrypt, decrypt ***)
+
+/// keygen: create a fresh key in the caller's region
+///         its ae log is initially empty
+let keygen ()
+  : ST key
+  (requires fun _ -> True)
+  (ensures  fun h0 k h1 ->
+    B.modifies B.loc_none h0 h1 /\
+    invariant k h1) =
+  let ke = CPA.keygen () in
+  let ka = MAC.keygen () in
+  Key ka ke
+
+
+/// encrypt:
+///       We return a cipher, preserve the invariant,
+///       and extend the log by exactly one entry
+let encrypt (k:key) (plain:Plain.plain)
+  : ST ae_cipher
+  (requires 
+    invariant k)
+  (ensures  fun h0 c h1 ->
+    invariant k h1 /\
+    B.modifies (B.loc_union (B.loc_mreference k.mac.MAC.log)
+                            (B.loc_mreference k.enc.CPA.log)) h0 h1 /\
+    (ae ==> ae_log k h1 == Seq.snoc (ae_log k h0) (plain, c))) =
+  let h0 = FStar.HyperStack.ST.get () in
+  let c = CPA.encrypt k.enc plain in
+  let h1 = FStar.HyperStack.ST.get () in
+  let t = MAC.mac k.mac c in
+  let h2 = get () in
+  assert (cpa_log h2 k == cpa_log h1 k);
+  assert (CPA.invariant k.enc h2); 
+  assert (MAC.invariant k.mac h2); 
+  mac_only_cpa_ciphers_snoc (mac_log h0 k) (MAC.Entry c t)
+                            (cpa_log h0 k) (CPA.Entry plain c);
+  if ae then 
+    composite_log_snoc (mac_log h0 k)  (MAC.Entry c t)
+                       (cpa_log h0 k) (CPA.Entry plain c);
+  (c, t)
+
+/// decrypt:
+///     In the ideal case, we prove it functionally correct and secure
+///     meaning that we the plain text returned is exactly the one in in AE log
+let decrypt (k:key) (c:ae_cipher)
+  : ST (option Plain.plain)
+  (requires 
+    invariant k)
+  (ensures fun h0 res h1 ->
+    invariant k h1 /\
+    h0 == h1 /\
+    (ae ==>
+     (match res with
+      | Some plain -> ae_log k h1 `Log.has` (plain, c)
+      | None -> True))) = //forall plain. ~ (ae_log k h1 `Log.has` (plain, c))))) =
+  let h = get() in
+  let c, tag = c in
+  if MAC.verify k.mac c tag
+  then begin
+       if ae then mac_only_cpa_ciphers_mem (mac_log h k) (cpa_log h k) (c, tag);
+       let p = CPA.decrypt k.enc c in
+       if ae then invert_invariant h k (c,tag) p;
+       Some p
+  end
+  else None
+
